\documentclass[12pt]{article}
\usepackage{amsmath}
\usepackage{xcolor}
\begin{document}
\documentclass[12pt]{article}
\usepackage{amsmath, amssymb, xcolor}
\usepackage[margin=1in]{geometry}
\setlength{\parindent}{0pt}
\setlength{\parskip}{0.5em}
\begin{document}
\begin{center}
\Large\textbf{Vector Space Proof Demonstration}\\[0.5em]
\normalsize\textit{Generated by the Khwarizmi Symbolic System}\\[1em]
\end{center}
\textbf{Goal:} Prove that $(2 \cdot (u + 0) + -1 \cdot u) = u$.
\\[1em]
\textbf{Proof:}
\\[0.5em]
\begin{alignat*}{3}
(2)\;& (u + 0) = u & \quad\textcolor{gray}{[VS\_Add\_Id]} \\
(2a)\;& 2 \cdot (u + 0) = 2 \cdot u & \quad\textcolor{gray}{[VS\_Add\_Id]} \\
(2b)\;& (2 \cdot (u + 0) + -1 \cdot u) = (2 \cdot u + -1 \cdot u) & \quad\textcolor{gray}{[VS\_Add\_Id]} \\
(3)\;& (2 \cdot u + -1 \cdot u) = (2 + -1) \cdot u & \quad\textcolor{gray}{[VS\_Factor\_Scalar]} \\
(4)\;& (2 + -1) = 1 & \quad\textcolor{gray}{[Scalar\_Arith]} \\
(4a)\;& (2 + -1) \cdot u = 1 \cdot u & \quad\textcolor{gray}{[Scalar\_Arith]} \\
(5)\;& 1 \cdot u = u & \quad\textcolor{gray}{[VS\_Scalar\_Id]} \\
\\[1em]
&\textbf{Hence, } u =  u\\[1em]
\end{alignat*}
\vfill
\begin{center}
\small\textit{Proof log automatically generated by Khwarizmi. All transformations follow registered axioms.}
\end{center}
\end{document}
\end{document}